Test/og/DeviceCache.bpl
@@ -3,10 +3,10 @@
 type X;
 function {:builtin "MapConst"} mapconstbool(bool): [X]bool;
 const nil: X;
-var {:phase 1} ghostLock: X;
-var {:phase 1} lock: X;
-var {:phase 1} currsize: int;
-var {:phase 1} newsize: int;
+var {:layer 1} ghostLock: X;
+var {:layer 1} lock: X;
+var {:layer 1} currsize: int;
+var {:layer 1} newsize: int;
 
 function {:builtin "MapConst"} MapConstBool(bool) : [X]bool;
 function {:inline} {:linear "tid"} TidCollector(x: X) : [X]bool
@@ -24,27 +24,27 @@ function {:inline} Inv(ghostLock: X, currsize: int, newsize: int) : (bool)
     (ghostLock == nil <==> currsize == newsize)
 }
 
-procedure {:yields} {:phase 1} YieldToReadCache({:linear "tid"} tid: X)
-requires {:phase 1} Inv(ghostLock, currsize, newsize) && tid != nil;
-ensures {:phase 1} Inv(ghostLock, currsize, newsize) && old(currsize) <= currsize;
+procedure {:yields} {:layer 1} YieldToReadCache({:linear "tid"} tid: X)
+requires {:layer 1} Inv(ghostLock, currsize, newsize) && tid != nil;
+ensures {:layer 1} Inv(ghostLock, currsize, newsize) && old(currsize) <= currsize;
 {
    yield;
-   assert {:phase 1} Inv(ghostLock, currsize, newsize) && old(currsize) <= currsize;
+   assert {:layer 1} Inv(ghostLock, currsize, newsize) && old(currsize) <= currsize;
 }
 
-procedure {:yields} {:phase 1} YieldToWriteCache({:linear "tid"} tid: X)
-requires {:phase 1} Inv(ghostLock, currsize, newsize) && ghostLock == tid && tid != nil;
-ensures {:phase 1} Inv(ghostLock, currsize, newsize) && ghostLock == tid && old(currsize) == currsize && old(newsize) == newsize;
+procedure {:yields} {:layer 1} YieldToWriteCache({:linear "tid"} tid: X)
+requires {:layer 1} Inv(ghostLock, currsize, newsize) && ghostLock == tid && tid != nil;
+ensures {:layer 1} Inv(ghostLock, currsize, newsize) && ghostLock == tid && old(currsize) == currsize && old(newsize) == newsize;
 {
     yield;
-    assert {:phase 1} Inv(ghostLock, currsize, newsize) && tid != nil && ghostLock == tid && old(currsize) == currsize && old(newsize) == newsize;
+    assert {:layer 1} Inv(ghostLock, currsize, newsize) && tid != nil && ghostLock == tid && old(currsize) == currsize && old(newsize) == newsize;
 }
 
 procedure Allocate({:linear_in "tid"} xls': [X]bool) returns ({:linear "tid"} xls: [X]bool, {:linear "tid"} xl: X);
-ensures {:phase 1} xl != nil;
+ensures {:layer 1} xl != nil;
 
-procedure {:yields} {:phase 1} main({:linear_in "tid"} xls':[X]bool)
-requires {:phase 1} xls' == mapconstbool(true);
+procedure {:yields} {:layer 1} main({:linear_in "tid"} xls':[X]bool)
+requires {:layer 1} xls' == mapconstbool(true);
 {
     var {:linear "tid"} tid: X;
     var {:linear "tid"} xls: [X]bool;
@@ -55,24 +55,24 @@ requires {:phase 1} xls' == mapconstbool(true);
     call Init(xls);
     
     yield;
-    assert {:phase 1} Inv(ghostLock, currsize, newsize);
+    assert {:layer 1} Inv(ghostLock, currsize, newsize);
 
     while (*)
-    invariant {:phase 1} Inv(ghostLock, currsize, newsize);
+    invariant {:layer 1} Inv(ghostLock, currsize, newsize);
     {
         call xls, tid := Allocate(xls);
 	yield;
-    	assert {:phase 1} Inv(ghostLock, currsize, newsize);
+    	assert {:layer 1} Inv(ghostLock, currsize, newsize);
         async call Thread(tid);
 	yield;
-    	assert {:phase 1} Inv(ghostLock, currsize, newsize);
+    	assert {:layer 1} Inv(ghostLock, currsize, newsize);
     }
     yield;
 }
 
-procedure {:yields} {:phase 1} Thread({:linear "tid"} tid: X)
-requires {:phase 1} tid != nil;
-requires {:phase 1} Inv(ghostLock, currsize, newsize);
+procedure {:yields} {:layer 1} Thread({:linear "tid"} tid: X)
+requires {:layer 1} tid != nil;
+requires {:layer 1} Inv(ghostLock, currsize, newsize);
 {
     var start, size, bytesRead: int;
 
@@ -81,11 +81,11 @@ requires {:phase 1} Inv(ghostLock, currsize, newsize);
     call bytesRead := Read(tid, start, size);
 }
 
-procedure {:yields} {:phase 1} Read({:linear "tid"} tid: X, start : int, size : int) returns (bytesRead : int)
-requires {:phase 1} tid != nil;
-requires {:phase 1} 0 <= start && 0 <= size;
-requires {:phase 1} Inv(ghostLock, currsize, newsize);
-ensures {:phase 1} 0 <= bytesRead && bytesRead <= size;
+procedure {:yields} {:layer 1} Read({:linear "tid"} tid: X, start : int, size : int) returns (bytesRead : int)
+requires {:layer 1} tid != nil;
+requires {:layer 1} 0 <= start && 0 <= size;
+requires {:layer 1} Inv(ghostLock, currsize, newsize);
+ensures {:layer 1} 0 <= bytesRead && bytesRead <= size;
 {
     var i, tmp: int;
 
@@ -121,19 +121,19 @@ COPY_TO_BUFFER:
     call ReadCache(tid, start, bytesRead);
 }
 
-procedure {:yields} {:phase 1} WriteCache({:linear "tid"} tid: X, index: int)
-requires {:phase 1} Inv(ghostLock, currsize, newsize);
-requires {:phase 1} ghostLock == tid && tid != nil;
-ensures {:phase 1} ghostLock == tid;
-ensures {:phase 1} Inv(ghostLock, currsize, newsize) && old(currsize) == currsize && old(newsize) == newsize;
+procedure {:yields} {:layer 1} WriteCache({:linear "tid"} tid: X, index: int)
+requires {:layer 1} Inv(ghostLock, currsize, newsize);
+requires {:layer 1} ghostLock == tid && tid != nil;
+ensures {:layer 1} ghostLock == tid;
+ensures {:layer 1} Inv(ghostLock, currsize, newsize) && old(currsize) == currsize && old(newsize) == newsize;
 {
     var j: int;
 
     par YieldToWriteCache(tid);
     call j := ReadCurrsize(tid);
     while (j < index)
-    invariant {:phase 1} ghostLock == tid && currsize <= j && tid == tid;
-    invariant {:phase 1} Inv(ghostLock, currsize, newsize) && old(currsize) == currsize && old(newsize) == newsize;
+    invariant {:layer 1} ghostLock == tid && currsize <= j && tid == tid;
+    invariant {:layer 1} Inv(ghostLock, currsize, newsize) && old(currsize) == currsize && old(newsize) == newsize;
     {
         par YieldToWriteCache(tid);
         call WriteCacheEntry(tid, j);
@@ -142,12 +142,12 @@ ensures {:phase 1} Inv(ghostLock, currsize, newsize) && old(currsize) == currsiz
     par YieldToWriteCache(tid);
 }
 
-procedure {:yields} {:phase 1} ReadCache({:linear "tid"} tid: X, start: int, bytesRead: int)
-requires {:phase 1} Inv(ghostLock, currsize, newsize);
-requires {:phase 1} tid != nil;
-requires {:phase 1} 0 <= start && 0 <= bytesRead;
-requires {:phase 1} (bytesRead == 0 || start + bytesRead <= currsize);
-ensures {:phase 1} Inv(ghostLock, currsize, newsize);
+procedure {:yields} {:layer 1} ReadCache({:linear "tid"} tid: X, start: int, bytesRead: int)
+requires {:layer 1} Inv(ghostLock, currsize, newsize);
+requires {:layer 1} tid != nil;
+requires {:layer 1} 0 <= start && 0 <= bytesRead;
+requires {:layer 1} (bytesRead == 0 || start + bytesRead <= currsize);
+ensures {:layer 1} Inv(ghostLock, currsize, newsize);
 {
     var j: int;
 
@@ -155,11 +155,11 @@ ensures {:phase 1} Inv(ghostLock, currsize, newsize);
 
     j := 0;
     while(j < bytesRead)
-    invariant {:phase 1} 0 <= j;
-    invariant {:phase 1} bytesRead == 0 || start + bytesRead <= currsize; 
-    invariant {:phase 1} Inv(ghostLock, currsize, newsize);
+    invariant {:layer 1} 0 <= j;
+    invariant {:layer 1} bytesRead == 0 || start + bytesRead <= currsize; 
+    invariant {:layer 1} Inv(ghostLock, currsize, newsize);
     {
-	assert {:phase 1} start + j < currsize;
+	assert {:layer 1} start + j < currsize;
         call ReadCacheEntry(tid, start + j);
         j := j + 1;
 	par YieldToReadCache(tid);
@@ -168,29 +168,29 @@ ensures {:phase 1} Inv(ghostLock, currsize, newsize);
     par YieldToReadCache(tid);
 }
 
-procedure {:yields} {:phase 0,1} Init({:linear "tid"} xls:[X]bool);
+procedure {:yields} {:layer 0,1} Init({:linear "tid"} xls:[X]bool);
 ensures {:atomic} |{ A: assert xls == mapconstbool(true); currsize := 0; newsize := 0; lock := nil; ghostLock := nil; return true; }|;
 
-procedure {:yields} {:phase 0,1} ReadCurrsize({:linear "tid"} tid: X) returns (val: int);
+procedure {:yields} {:layer 0,1} ReadCurrsize({:linear "tid"} tid: X) returns (val: int);
 ensures {:right} |{A: assert tid != nil; assert lock == tid || ghostLock == tid; val := currsize; return true; }|;
 
-procedure {:yields} {:phase 0,1} ReadNewsize({:linear "tid"} tid: X) returns (val: int);
+procedure {:yields} {:layer 0,1} ReadNewsize({:linear "tid"} tid: X) returns (val: int);
 ensures {:right} |{A: assert tid != nil; assert lock == tid || ghostLock == tid; val := newsize; return true; }|;
 
-procedure {:yields} {:phase 0,1} WriteNewsize({:linear "tid"} tid: X, val: int);
+procedure {:yields} {:layer 0,1} WriteNewsize({:linear "tid"} tid: X, val: int);
 ensures {:atomic} |{A: assert tid != nil; assert lock == tid && ghostLock == nil; newsize := val; ghostLock := tid; return true; }|;
 
-procedure {:yields} {:phase 0,1} WriteCurrsize({:linear "tid"} tid: X, val: int);
+procedure {:yields} {:layer 0,1} WriteCurrsize({:linear "tid"} tid: X, val: int);
 ensures {:atomic} |{A: assert tid != nil; assert lock == tid && ghostLock == tid; currsize := val; ghostLock := nil; return true; }|;
 
-procedure {:yields} {:phase 0,1} ReadCacheEntry({:linear "tid"} tid: X, index: int);
+procedure {:yields} {:layer 0,1} ReadCacheEntry({:linear "tid"} tid: X, index: int);
 ensures {:atomic} |{ A: assert 0 <= index && index < currsize; return true; }|;
 
-procedure {:yields} {:phase 0,1} WriteCacheEntry({:linear "tid"} tid: X, index: int);
+procedure {:yields} {:layer 0,1} WriteCacheEntry({:linear "tid"} tid: X, index: int);
 ensures {:right} |{ A: assert tid != nil; assert currsize <= index && ghostLock == tid; return true; }|;
 
-procedure {:yields} {:phase 0,1} acquire({:linear "tid"} tid: X);
+procedure {:yields} {:layer 0,1} acquire({:linear "tid"} tid: X);
 ensures {:right} |{ A: assert tid != nil; assume lock == nil; lock := tid; return true; }|;
 
-procedure {:yields} {:phase 0,1} release({:linear "tid"} tid: X);
+procedure {:yields} {:layer 0,1} release({:linear "tid"} tid: X);
 ensures {:left} |{ A: assert tid != nil; assert lock == tid; lock := nil; return true; }|;
