Test/og/Program5.bpl
@@ -5,8 +5,8 @@ const unique nil: Tid;
 function {:builtin "MapConst"} MapConstBool(bool): [Tid]bool;
 function {:builtin "MapOr"} MapOr([Tid]bool, [Tid]bool) : [Tid]bool;
 
-var {:phase 0,3} Color:int;
-var {:phase 0,3} lock:Tid;
+var {:layer 0,3} Color:int;
+var {:layer 0,3} lock:Tid;
 
 function {:inline} {:linear "tid"} TidCollector(x: Tid) : [Tid]bool
 {
@@ -26,14 +26,14 @@ function {:inline} White(i:int) returns(bool) { i == 1 }
 function {:inline} Gray(i:int) returns(bool) { i == 2 }
 function {:inline} Black(i:int) returns(bool) { i >= 3 }
 
-procedure {:yields} {:phase 2} YieldColorOnlyGetsDarker()
-ensures {:phase 2} Color >= old(Color);
+procedure {:yields} {:layer 2} YieldColorOnlyGetsDarker()
+ensures {:layer 2} Color >= old(Color);
 {
   yield;
-  assert {:phase 2} Color >= old(Color);
+  assert {:layer 2} Color >= old(Color);
 }
 
-procedure {:yields} {:phase 2,3} TopWriteBarrier({:linear "tid"} tid:Tid)
+procedure {:yields} {:layer 2,3} TopWriteBarrier({:linear "tid"} tid:Tid)
 ensures {:atomic} |{ A: assert tid != nil; goto B, C; 
                      B: assume White(Color); Color := GRAY(); return true; 
                      C: return true;}|;
@@ -46,7 +46,7 @@ ensures {:atomic} |{ A: assert tid != nil; goto B, C;
   yield;
 }
 
-procedure {:yields} {:phase 1,2} MidWriteBarrier({:linear "tid"} tid:Tid)
+procedure {:yields} {:layer 1,2} MidWriteBarrier({:linear "tid"} tid:Tid)
 ensures {:atomic} |{ A: assert tid != nil; goto B, C; 
                      B: assume White(Color); Color := GRAY(); return true; 
                      C: return true; }|;
@@ -60,18 +60,18 @@ ensures {:atomic} |{ A: assert tid != nil; goto B, C;
        yield;
 }
 
-procedure {:yields} {:phase 0,1} AcquireLock({:linear "tid"} tid: Tid);
+procedure {:yields} {:layer 0,1} AcquireLock({:linear "tid"} tid: Tid);
   ensures {:right} |{ A: assert tid != nil; assume lock == nil; lock := tid; return true; }|;
 
-procedure {:yields} {:phase 0,1} ReleaseLock({:linear "tid"} tid: Tid);
+procedure {:yields} {:layer 0,1} ReleaseLock({:linear "tid"} tid: Tid);
   ensures {:left} |{ A: assert tid != nil; assert lock == tid; lock := nil; return true; }|;
 
-procedure {:yields} {:phase 0,1} SetColorLocked({:linear "tid"} tid:Tid, newCol:int); 
+procedure {:yields} {:layer 0,1} SetColorLocked({:linear "tid"} tid:Tid, newCol:int); 
   ensures {:atomic} |{A: assert tid != nil; assert lock == tid; Color := newCol; return true;}|;
 
-procedure {:yields} {:phase 0,1} GetColorLocked({:linear "tid"} tid:Tid) returns (col:int);
+procedure {:yields} {:layer 0,1} GetColorLocked({:linear "tid"} tid:Tid) returns (col:int);
   ensures {:both} |{A: assert tid != nil; assert lock == tid; col := Color; return true;}|;
 
-procedure {:yields} {:phase 1,2} GetColorNoLock() returns (col:int);
+procedure {:yields} {:layer 1,2} GetColorNoLock() returns (col:int);
   ensures {:atomic} |{A: col := Color; return true;}|;
 
