Test/og/ticket.bpl
@@ -8,10 +8,10 @@ axiom (forall x: int, y: int :: RightClosed(x)[y] <==> y <= x);
 type X;
 function {:builtin "MapConst"} mapconstbool(bool): [X]bool;
 const nil: X;
-var {:phase 2} t: int;
-var {:phase 2} s: int;
-var {:phase 2} cs: X;
-var {:phase 2} T: [int]bool;
+var {:layer 2} t: int;
+var {:layer 2} s: int;
+var {:layer 2} cs: X;
+var {:layer 2} T: [int]bool;
 
 function {:builtin "MapConst"} MapConstBool(bool) : [X]bool;
 function {:inline} {:linear "tid"} TidCollector(x: X) : [X]bool
@@ -34,10 +34,10 @@ function {:inline} Inv2(tickets: [int]bool, ticket: int, lock: X): (bool)
 }
 
 procedure Allocate({:linear_in "tid"} xls':[X]bool) returns ({:linear "tid"} xls: [X]bool, {:linear "tid"} xl: X);
-ensures {:phase 1} {:phase 2} xl != nil;
+ensures {:layer 1} {:layer 2} xl != nil;
 
-procedure {:yields} {:phase 2} main({:linear_in "tid"} xls':[X]bool)
-requires {:phase 2} xls' == mapconstbool(true);
+procedure {:yields} {:layer 2} main({:linear_in "tid"} xls':[X]bool)
+requires {:layer 2} xls' == mapconstbool(true);
 {
     var {:linear "tid"} tid: X;
     var {:linear "tid"} xls: [X]bool;
@@ -50,8 +50,8 @@ requires {:phase 2} xls' == mapconstbool(true);
     par Yield1() | Yield2();
 
     while (*)
-    invariant {:phase 1} Inv1(T, t);
-    invariant {:phase 2} Inv2(T, s, cs);
+    invariant {:layer 1} Inv1(T, t);
+    invariant {:layer 2} Inv2(T, s, cs);
     {
         call xls, tid := Allocate(xls);
         async call Customer(tid);
@@ -60,14 +60,14 @@ requires {:phase 2} xls' == mapconstbool(true);
     par Yield1() | Yield2();
 }
 
-procedure {:yields} {:phase 2} Customer({:linear_in "tid"} tid: X)
-requires {:phase 1} Inv1(T, t);
-requires {:phase 2} tid != nil && Inv2(T, s, cs);
+procedure {:yields} {:layer 2} Customer({:linear_in "tid"} tid: X)
+requires {:layer 1} Inv1(T, t);
+requires {:layer 2} tid != nil && Inv2(T, s, cs);
 {
     par Yield1() | Yield2();    
     while (*) 
-    invariant {:phase 1} Inv1(T, t);
-    invariant {:phase 2} Inv2(T, s, cs);
+    invariant {:layer 1} Inv1(T, t);
+    invariant {:layer 2} Inv2(T, s, cs);
     {
         call Enter(tid);
         par Yield1() | Yield2() | YieldSpec(tid);
@@ -77,11 +77,11 @@ requires {:phase 2} tid != nil && Inv2(T, s, cs);
     par Yield1() | Yield2();
 }
 
-procedure {:yields} {:phase 2} Enter({:linear "tid"} tid: X)
-requires {:phase 1} Inv1(T, t);
-ensures {:phase 1} Inv1(T,t);
-requires {:phase 2} tid != nil && Inv2(T, s, cs);
-ensures {:phase 2} Inv2(T, s, cs) && cs == tid;
+procedure {:yields} {:layer 2} Enter({:linear "tid"} tid: X)
+requires {:layer 1} Inv1(T, t);
+ensures {:layer 1} Inv1(T,t);
+requires {:layer 2} tid != nil && Inv2(T, s, cs);
+ensures {:layer 2} Inv2(T, s, cs) && cs == tid;
 {
     var m: int;
 
@@ -92,9 +92,9 @@ ensures {:phase 2} Inv2(T, s, cs) && cs == tid;
     par Yield1() | Yield2() | YieldSpec(tid);
 }
 
-procedure {:yields} {:phase 1,2} GetTicketAbstract({:linear "tid"} tid: X) returns (m: int)
-requires {:phase 1} Inv1(T, t);
-ensures {:phase 1} Inv1(T, t);
+procedure {:yields} {:layer 1,2} GetTicketAbstract({:linear "tid"} tid: X) returns (m: int)
+requires {:layer 1} Inv1(T, t);
+ensures {:layer 1} Inv1(T, t);
 ensures {:right} |{ A: havoc m, t; assume !T[m]; T[m] := true; return true; }|;
 {
     par Yield1();
@@ -102,39 +102,39 @@ ensures {:right} |{ A: havoc m, t; assume !T[m]; T[m] := true; return true; }|;
     par Yield1();
 }
 
-procedure {:yields} {:phase 2} YieldSpec({:linear "tid"} tid: X)
-requires {:phase 2} tid != nil && cs == tid;
-ensures {:phase 2} cs == tid;
+procedure {:yields} {:layer 2} YieldSpec({:linear "tid"} tid: X)
+requires {:layer 2} tid != nil && cs == tid;
+ensures {:layer 2} cs == tid;
 {
     yield;
-    assert {:phase 2} tid != nil && cs == tid;
+    assert {:layer 2} tid != nil && cs == tid;
 }
 
-procedure {:yields} {:phase 2} Yield2()
-requires {:phase 2} Inv2(T, s, cs);
-ensures {:phase 2} Inv2(T, s, cs);
+procedure {:yields} {:layer 2} Yield2()
+requires {:layer 2} Inv2(T, s, cs);
+ensures {:layer 2} Inv2(T, s, cs);
 {
     yield;
-    assert {:phase 2} Inv2(T, s, cs);
+    assert {:layer 2} Inv2(T, s, cs);
 }
 
-procedure {:yields} {:phase 1} Yield1()
-requires {:phase 1} Inv1(T, t);
-ensures {:phase 1} Inv1(T,t);
+procedure {:yields} {:layer 1} Yield1()
+requires {:layer 1} Inv1(T, t);
+ensures {:layer 1} Inv1(T,t);
 {
     yield;
-    assert {:phase 1} Inv1(T,t);
+    assert {:layer 1} Inv1(T,t);
 }
 
-procedure {:yields} {:phase 0,2} Init({:linear "tid"} xls:[X]bool);
+procedure {:yields} {:layer 0,2} Init({:linear "tid"} xls:[X]bool);
 ensures {:atomic} |{ A: assert xls == mapconstbool(true); cs := nil; t := 0; s := 0; T := RightOpen(0); return true; }|;
 
-procedure {:yields} {:phase 0,1} GetTicket({:linear "tid"} tid: X) returns (m: int);
+procedure {:yields} {:layer 0,1} GetTicket({:linear "tid"} tid: X) returns (m: int);
 ensures {:atomic} |{ A: m := t; t := t + 1; T[m] := true; return true; }|;
 
-procedure {:yields} {:phase 0,2} WaitAndEnter({:linear "tid"} tid: X, m:int);
+procedure {:yields} {:layer 0,2} WaitAndEnter({:linear "tid"} tid: X, m:int);
 ensures {:atomic} |{ A: assume m <= s; cs := tid; return true; }|;
 
-procedure {:yields} {:phase 0,2} Leave({:linear "tid"} tid: X);
+procedure {:yields} {:layer 0,2} Leave({:linear "tid"} tid: X);
 ensures {:atomic} |{ A: s := s + 1; cs := nil; return true; }|;
 
