Test/og/FlanaganQadeer.bpl
@@ -2,8 +2,8 @@
 // RUN: %diff "%s.expect" "%t"
 type X;
 const nil: X;
-var {:phase 1} l: X;
-var {:phase 1} x: int;
+var {:layer 1} l: X;
+var {:layer 1} x: int;
 
 function {:builtin "MapConst"} MapConstBool(bool) : [X]bool;
 function {:inline} {:linear "tid"} TidCollector(x: X) : [X]bool
@@ -12,9 +12,9 @@ function {:inline} {:linear "tid"} TidCollector(x: X) : [X]bool
 }
 
 procedure Allocate() returns ({:linear "tid"} xls: X);
-ensures {:phase 1} xls != nil;
+ensures {:layer 1} xls != nil;
 
-procedure {:yields} {:phase 1} main()
+procedure {:yields} {:layer 1} main()
 {
     var {:linear "tid"} tid: X;
     var val: int;
@@ -29,17 +29,17 @@ procedure {:yields} {:phase 1} main()
     }
     yield;
 }
-procedure {:yields} {:phase 0,1} Lock(tid: X);
+procedure {:yields} {:layer 0,1} Lock(tid: X);
 ensures {:atomic} |{A: assume l == nil; l := tid; return true; }|;
 
-procedure {:yields} {:phase 0,1} Unlock();
+procedure {:yields} {:layer 0,1} Unlock();
 ensures {:atomic} |{A: l := nil; return true; }|;
 
-procedure {:yields} {:phase 0,1} Set(val: int);
+procedure {:yields} {:layer 0,1} Set(val: int);
 ensures {:atomic} |{A: x := val; return true; }|;
 
-procedure {:yields} {:phase 1} foo({:linear_in "tid"} tid': X, val: int)
-requires {:phase 1} tid' != nil;
+procedure {:yields} {:layer 1} foo({:linear_in "tid"} tid': X, val: int)
+requires {:layer 1} tid' != nil;
 {
     var {:linear "tid"} tid: X;
     tid := tid';
@@ -49,19 +49,19 @@ requires {:phase 1} tid' != nil;
     call tid := Yield(tid);
     call Set(val);
     call tid := Yield(tid);
-    assert {:phase 1} x == val;
+    assert {:layer 1} x == val;
     call tid := Yield(tid);
     call Unlock();
     yield;
 }
 
-procedure {:yields} {:phase 1} Yield({:linear_in "tid"} tid': X) returns ({:linear "tid"} tid: X)
-requires {:phase 1} tid' != nil;
-ensures {:phase 1} tid == tid';
-ensures {:phase 1} old(l) == tid ==> old(l) == l && old(x) == x;
+procedure {:yields} {:layer 1} Yield({:linear_in "tid"} tid': X) returns ({:linear "tid"} tid: X)
+requires {:layer 1} tid' != nil;
+ensures {:layer 1} tid == tid';
+ensures {:layer 1} old(l) == tid ==> old(l) == l && old(x) == x;
 {
     tid := tid';
     yield;
-    assert {:phase 1} tid != nil;
-    assert {:phase 1} (old(l) == tid ==> old(l) == l && old(x) == x);
+    assert {:layer 1} tid != nil;
+    assert {:layer 1} (old(l) == tid ==> old(l) == l && old(x) == x);
 }
