Test/og/Program3.bpl
@@ -1,17 +1,17 @@
 // RUN: %boogie -noinfer -typeEncoding:m -useArrayTheory "%s" > "%t"
 // RUN: %diff "%s.expect" "%t"
-var {:phase 1} x:int;
+var {:layer 1} x:int;
 
-procedure {:yields} {:phase 1} yield_x()
-ensures {:phase 1} x >= old(x); 
+procedure {:yields} {:layer 1} yield_x()
+ensures {:layer 1} x >= old(x); 
 {
     yield;
-    assert {:phase 1} x >= old(x);
+    assert {:layer 1} x >= old(x);
 }
 
-procedure {:yields} {:phase 1} p() 
-requires {:phase 1} x >= 5; 
-ensures {:phase 1} x >= 8; 
+procedure {:yields} {:layer 1} p() 
+requires {:layer 1} x >= 5; 
+ensures {:layer 1} x >= 8; 
 { 
     call yield_x();
     call Incr(1); 
@@ -22,14 +22,14 @@ ensures {:phase 1} x >= 8;
     call yield_x();
 }
 
-procedure {:yields} {:phase 1} q() 
+procedure {:yields} {:layer 1} q() 
 { 
     yield;
     call Incr(3); 
     yield;
 }
 
-procedure {:yields} {:phase 0,1} Incr(val: int);
+procedure {:yields} {:layer 0,1} Incr(val: int);
 ensures {:atomic}
 |{A:
   x := x + val; return true;
