Test/og/Program4.bpl
@@ -13,11 +13,11 @@ function {:inline} {:linear "tid"} TidSetCollector(x: [Tid]bool) : [Tid]bool
   x
 }
 
-var {:phase 1} a:[Tid]int;
+var {:layer 1} a:[Tid]int;
 
 procedure Allocate() returns ({:linear "tid"} tid:Tid); 
 
-procedure {:yields} {:phase 1} main() { 
+procedure {:yields} {:layer 1} main() { 
     var {:linear "tid"} tid:Tid;
 
     yield;
@@ -29,28 +29,28 @@ procedure {:yields} {:phase 1} main() {
     yield;
 }
 
-procedure {:yields} {:phase 1} P({:linear "tid"} tid: Tid) 
-ensures {:phase 1} a[tid] == old(a)[tid] + 1; 
+procedure {:yields} {:layer 1} P({:linear "tid"} tid: Tid) 
+ensures {:layer 1} a[tid] == old(a)[tid] + 1; 
 { 
     var t:int;
 
     yield;
-    assert {:phase 1} a[tid] == old(a)[tid];
+    assert {:layer 1} a[tid] == old(a)[tid];
     call t := Read(tid); 
     yield;
-    assert {:phase 1} a[tid] == t; 
+    assert {:layer 1} a[tid] == t; 
     call Write(tid, t + 1); 
     yield;
-    assert {:phase 1} a[tid] == t + 1; 
+    assert {:layer 1} a[tid] == t + 1; 
 }
 
-procedure {:yields} {:phase 0,1} Read({:linear "tid"} tid: Tid) returns (val: int);
+procedure {:yields} {:layer 0,1} Read({:linear "tid"} tid: Tid) returns (val: int);
 ensures {:atomic}
 |{A:
   val := a[tid]; return true;
 }|;
 
-procedure {:yields} {:phase 0,1} Write({:linear "tid"} tid: Tid, val: int);
+procedure {:yields} {:layer 0,1} Write({:linear "tid"} tid: Tid, val: int);
 ensures {:atomic}
 |{A:
   a[tid] := val; return true;
