Test/og/bar.bpl
@@ -1,47 +1,47 @@
 // RUN: %boogie -noinfer "%s" > "%t"
 // RUN: %diff "%s.expect" "%t"
-var {:phase 1} g:int;
+var {:layer 1} g:int;
 
-procedure {:yields} {:phase 1} PB()
+procedure {:yields} {:layer 1} PB()
 {
   yield;
   call Incr();
   yield;
 }
 
-procedure {:yields} {:phase 0,1} Incr();
+procedure {:yields} {:layer 0,1} Incr();
 ensures {:atomic}
 |{A:
   g := g + 1; return true;
 }|;
 
-procedure {:yields} {:phase 0,1} Set(v: int);
+procedure {:yields} {:layer 0,1} Set(v: int);
 ensures {:atomic}
 |{A:
   g := v; return true;
 }|;
 
-procedure {:yields} {:phase 1} PC()
-ensures {:phase 1} g == old(g);
+procedure {:yields} {:layer 1} PC()
+ensures {:layer 1} g == old(g);
 {
   yield;
-  assert {:phase 1} g == old(g);
+  assert {:layer 1} g == old(g);
 }
 
-procedure {:yields} {:phase 1} PE()
+procedure {:yields} {:layer 1} PE()
 {
   call PC();
 }
 
-procedure {:yields} {:phase 1} PD()
+procedure {:yields} {:layer 1} PD()
 {
   yield;
   call Set(3);
   call PC();
-  assert {:phase 1} g == 3;
+  assert {:layer 1} g == 3;
 }
 
-procedure {:yields} {:phase 1} Main2()
+procedure {:yields} {:layer 1} Main2()
 {
   yield;
   while (*)
