Test/og/lock.bpl
@@ -1,8 +1,8 @@
 // RUN: %boogie -noinfer -typeEncoding:m -useArrayTheory "%s" > "%t"
 // RUN: %diff "%s.expect" "%t"
-var {:phase 2} b: bool;
+var {:layer 2} b: bool;
 
-procedure {:yields} {:phase 2} main()
+procedure {:yields} {:layer 2} main()
 {
     yield;
     while (*)
@@ -13,7 +13,7 @@ procedure {:yields} {:phase 2} main()
     yield;
 }
 
-procedure {:yields} {:phase 2} Customer()
+procedure {:yields} {:layer 2} Customer()
 {
     yield;
     while (*) 
@@ -26,7 +26,7 @@ procedure {:yields} {:phase 2} Customer()
     yield;
 }
 
-procedure {:yields} {:phase 1,2} Enter() 
+procedure {:yields} {:layer 1,2} Enter() 
 ensures {:atomic} |{ A: assume !b; b := true; return true; }|;
 {
     var status: bool;
@@ -46,12 +46,12 @@ ensures {:atomic} |{ A: assume !b; b := true; return true; }|;
 	goto L;
 }
 
-procedure {:yields} {:phase 0,2} CAS(prev: bool, next: bool) returns (status: bool);
+procedure {:yields} {:layer 0,2} CAS(prev: bool, next: bool) returns (status: bool);
 ensures {:atomic} |{ 
 A: goto B, C; 
 B: assume b == prev; b := next; status := true; return true; 
 C: status := false; return true; 
 }|;
 
-procedure {:yields} {:phase 0,2} Leave();
+procedure {:yields} {:layer 0,2} Leave();
 ensures {:atomic} |{ A: b := false; return true; }|;
