Test/og/lock2.bpl
@@ -1,8 +1,8 @@
 // RUN: %boogie -noinfer -typeEncoding:m -useArrayTheory "%s" > "%t"
 // RUN: %diff "%s.expect" "%t"
-var {:phase 2} b: int;
+var {:layer 2} b: int;
 
-procedure {:yields} {:phase 2} main()
+procedure {:yields} {:layer 2} main()
 {
     yield;
     while (*)
@@ -13,7 +13,7 @@ procedure {:yields} {:phase 2} main()
     yield;
 }
 
-procedure {:yields} {:phase 2} Customer()
+procedure {:yields} {:layer 2} Customer()
 {
     yield;
     while (*) 
@@ -26,7 +26,7 @@ procedure {:yields} {:phase 2} Customer()
     yield;
 }
 
-procedure {:yields} {:phase 1,2} Enter() 
+procedure {:yields} {:layer 1,2} Enter() 
 ensures {:atomic} |{ A: assume b == 0; b := 1; return true; }|;
 {
     var _old, curr: int;
@@ -49,15 +49,15 @@ ensures {:atomic} |{ A: assume b == 0; b := 1; return true; }|;
     yield;
 }
 
-procedure {:yields} {:phase 0,2} Read() returns (val: int);
+procedure {:yields} {:layer 0,2} Read() returns (val: int);
 ensures {:atomic} |{ A: val := b; return true; }|;
 
-procedure {:yields} {:phase 0,2} CAS(prev: int, next: int) returns (_old: int);
+procedure {:yields} {:layer 0,2} CAS(prev: int, next: int) returns (_old: int);
 ensures {:atomic} |{ 
 A: _old := b; goto B, C; 
 B: assume _old == prev; b := next; return true; 
 C: assume _old != prev; return true; 
 }|;
 
-procedure {:yields} {:phase 0,2} Leave();
+procedure {:yields} {:layer 0,2} Leave();
 ensures {:atomic} |{ A: b := 0; return true; }|;
