Test/og/new1.bpl
@@ -2,7 +2,7 @@
 // RUN: %diff "%s.expect" "%t"
 function {:builtin "MapConst"} mapconstbool(x:bool): [int]bool;
 
-var {:phase 1} g:int;
+var {:layer 1} g:int;
 
 function {:inline} {:linear "Perm"} SetCollectorPerm(x: [int]bool) : [int]bool
 {
@@ -13,25 +13,25 @@ procedure Allocate_Perm({:linear_in "Perm"} Permissions: [int]bool) returns ({:l
 requires Permissions == mapconstbool(true);
 ensures xls == mapconstbool(true);
 
-procedure {:yields} {:phase 1} PB({:linear_in "Perm"} permVar_in:[int]bool)
-requires {:phase 1} permVar_in[0] && g == 0;
+procedure {:yields} {:layer 1} PB({:linear_in "Perm"} permVar_in:[int]bool)
+requires {:layer 1} permVar_in[0] && g == 0;
 {
   var {:linear "Perm"} permVar_out: [int]bool;
   permVar_out := permVar_in;
 
   yield;
-  assert {:phase 1} permVar_out[0];
-  assert {:phase 1} g == 0;
+  assert {:layer 1} permVar_out[0];
+  assert {:layer 1} g == 0;
 
   call IncrG();
 
   yield;
-  assert {:phase 1} permVar_out[0];
-  assert {:phase 1} g == 1;
+  assert {:layer 1} permVar_out[0];
+  assert {:layer 1} g == 1;
 }
 
-procedure {:yields} {:phase 1} Main({:linear_in "Perm"} Permissions: [int]bool)
-requires {:phase 0,1} Permissions == mapconstbool(true);
+procedure {:yields} {:layer 1} Main({:linear_in "Perm"} Permissions: [int]bool)
+requires {:layer 0,1} Permissions == mapconstbool(true);
 {
   var {:linear "Perm"} permVar_out: [int]bool;
 
@@ -42,8 +42,8 @@ requires {:phase 0,1} Permissions == mapconstbool(true);
   yield;
 }
 
-procedure {:yields} {:phase 0,1} SetG(val:int);
+procedure {:yields} {:layer 0,1} SetG(val:int);
 ensures {:atomic} |{A: g := val; return true; }|;
 
-procedure {:yields} {:phase 0,1} IncrG();
+procedure {:yields} {:layer 0,1} IncrG();
 ensures {:atomic} |{A: g := g + 1; return true; }|;
