Test/og/one.bpl
@@ -1,18 +1,18 @@
 // RUN: %boogie -noinfer "%s" > "%t"
 // RUN: %diff "%s.expect" "%t"
-var {:phase 1} x:int;
+var {:layer 1} x:int;
 
-procedure {:yields} {:phase 0,1} Set(v: int);
+procedure {:yields} {:layer 0,1} Set(v: int);
 ensures {:atomic}
 |{A:
   x := v; return true;
 }|;
 
-procedure {:yields} {:phase 1} B()
+procedure {:yields} {:layer 1} B()
 {
   yield;
   call Set(5);
   yield;
-  assert {:phase 1} x == 5;
+  assert {:layer 1} x == 5;
 }
 
