Test/og/t1.bpl
@@ -19,24 +19,24 @@ function {:inline} {:linear "2"} SetCollector2(x: [int]bool) : [int]bool
 }
 
 procedure Allocate() returns ({:linear "tid"} xls: int);
-ensures {:phase 1} xls != 0;
+ensures {:layer 1} xls != 0;
 
 procedure Allocate_1() returns ({:linear "1"} xls: [int]bool);
-ensures {:phase 1} xls == mapconstbool(true);
+ensures {:layer 1} xls == mapconstbool(true);
 
 procedure Allocate_2() returns ({:linear "2"} xls: [int]bool);
-ensures {:phase 1} xls == mapconstbool(true);
+ensures {:layer 1} xls == mapconstbool(true);
 
-var {:phase 1} g: int;
-var {:phase 1} h: int;
+var {:layer 1} g: int;
+var {:layer 1} h: int;
 
-procedure {:yields} {:phase 0,1} SetG(val:int);
+procedure {:yields} {:layer 0,1} SetG(val:int);
 ensures {:atomic} |{A: g := val; return true; }|;
 
-procedure {:yields} {:phase 0,1} SetH(val:int);
+procedure {:yields} {:layer 0,1} SetH(val:int);
 ensures {:atomic} |{A: h := val; return true; }|;
 
-procedure {:yields} {:phase 1} A({:linear_in "tid"} tid_in: int) returns ({:linear "tid"} tid_out: int) 
+procedure {:yields} {:layer 1} A({:linear_in "tid"} tid_in: int) returns ({:linear "tid"} tid_out: int) 
 {
     var {:linear "1"} x: [int]bool;
     var {:linear "2"} y: [int]bool;
@@ -48,22 +48,22 @@ procedure {:yields} {:phase 1} A({:linear_in "tid"} tid_in: int) returns ({:line
     yield;
     call SetG(0);
     yield;
-    assert {:phase 1} x == mapconstbool(true);    
-    assert {:phase 1} g == 0;    
+    assert {:layer 1} x == mapconstbool(true);    
+    assert {:layer 1} g == 0;    
 
     yield;
     call tid_child := Allocate();
     async call B(tid_child, x);
 
     yield;
-    assert {:phase 1} x == mapconstbool(true);    
-    assert {:phase 1} g == 0;
+    assert {:layer 1} x == mapconstbool(true);    
+    assert {:layer 1} g == 0;
 
     yield;
     call SetH(0);
 
     yield;
-    assert {:phase 1} h == 0 && y == mapconstbool(true);    
+    assert {:layer 1} h == 0 && y == mapconstbool(true);    
 
     yield;
     call tid_child := Allocate();
@@ -72,8 +72,8 @@ procedure {:yields} {:phase 1} A({:linear_in "tid"} tid_in: int) returns ({:line
     yield;
 }
 
-procedure {:yields} {:phase 1} B({:linear_in "tid"} tid_in: int, {:linear_in "1"} x_in: [int]bool) 
-requires {:phase 1} x_in != mapconstbool(false);
+procedure {:yields} {:layer 1} B({:linear_in "tid"} tid_in: int, {:linear_in "1"} x_in: [int]bool) 
+requires {:layer 1} x_in != mapconstbool(false);
 {
     var {:linear "tid"} tid_out: int;
     var {:linear "1"} x: [int]bool;
@@ -85,8 +85,8 @@ requires {:phase 1} x_in != mapconstbool(false);
     yield;
 }
 
-procedure {:yields} {:phase 1} C({:linear_in "tid"} tid_in: int, {:linear_in "2"} y_in: [int]bool) 
-requires {:phase 1} y_in != mapconstbool(false);
+procedure {:yields} {:layer 1} C({:linear_in "tid"} tid_in: int, {:linear_in "2"} y_in: [int]bool) 
+requires {:layer 1} y_in != mapconstbool(false);
 {
     var {:linear "tid"} tid_out: int;
     var {:linear "2"} y: [int]bool;
