Test/og/treiber-stack.bpl
@@ -16,24 +16,24 @@ axiom (forall x: lmap, i: Node, v: Node :: dom(Add(x, i, v)) == dom(x)[i:=true] 
 function Remove(x: lmap, i: Node): (lmap);
 axiom (forall x: lmap, i: Node :: dom(Remove(x, i)) == dom(x)[i:=false] && map(Remove(x, i)) == map(x));
 
-procedure {:yields} {:phase 0} ReadTopOfStack() returns (v:Node);
+procedure {:yields} {:layer 0} ReadTopOfStack() returns (v:Node);
 ensures {:right} |{ A: assume dom(Stack)[v] || dom(Used)[v]; return true; }|;
 
-procedure {:yields} {:phase 0} Load(i:Node) returns (v:Node);
+procedure {:yields} {:layer 0} Load(i:Node) returns (v:Node);
 ensures {:right} |{ A: assert dom(Stack)[i] || dom(Used)[i]; goto B,C;
 	            B: assume dom(Stack)[i]; v := map(Stack)[i]; return true; 
 		    C: assume !dom(Stack)[i]; return true; }|;
 
-procedure {:yields} {:phase 0} Store({:linear_in "Node"} l_in:lmap, i:Node, v:Node) returns ({:linear "Node"} l_out:lmap);
+procedure {:yields} {:layer 0} Store({:linear_in "Node"} l_in:lmap, i:Node, v:Node) returns ({:linear "Node"} l_out:lmap);
 ensures {:both} |{ A: assert dom(l_in)[i]; l_out := Add(l_in, i, v); return true; }|;
 
-procedure {:yields} {:phase 0} TransferToStack(oldVal: Node, newVal: Node, {:linear_in "Node"} l_in:lmap) returns (r: bool, {:linear "Node"} l_out:lmap);
+procedure {:yields} {:layer 0} TransferToStack(oldVal: Node, newVal: Node, {:linear_in "Node"} l_in:lmap) returns (r: bool, {:linear "Node"} l_out:lmap);
 ensures {:atomic} |{ A: assert dom(l_in)[newVal];
 		        goto B,C;
                         B: assume oldVal == TopOfStack; TopOfStack := newVal; l_out := EmptyLmap(); Stack := Add(Stack, newVal, map(l_in)[newVal]); r := true; return true;
 			C: assume oldVal != TopOfStack; l_out := l_in; r := false; return true; }|;
 
-procedure {:yields} {:phase 0} TransferFromStack(oldVal: Node, newVal: Node) returns (r: bool);
+procedure {:yields} {:layer 0} TransferFromStack(oldVal: Node, newVal: Node) returns (r: bool);
 ensures {:atomic} |{ A: goto B,C;
                         B: assume oldVal == TopOfStack; TopOfStack := newVal; Used := Add(Used, oldVal, map(Stack)[oldVal]); Stack := Remove(Stack, oldVal); r := true; return true;
 		        C: assume oldVal != TopOfStack; r := false; return true; }|;
@@ -50,10 +50,10 @@ function {:inline} Inv(TopOfStack: Node, Stack: lmap) : (bool)
 
 var {:linear "Node"} Used: lmap;
 
-procedure {:yields} {:phase 1} push(x: Node, {:linear_in "Node"} x_lmap: lmap)
-requires {:phase 1} dom(x_lmap)[x];
-requires {:phase 1} Inv(TopOfStack, Stack);
-ensures {:phase 1} Inv(TopOfStack, Stack);
+procedure {:yields} {:layer 1} push(x: Node, {:linear_in "Node"} x_lmap: lmap)
+requires {:layer 1} dom(x_lmap)[x];
+requires {:layer 1} Inv(TopOfStack, Stack);
+ensures {:layer 1} Inv(TopOfStack, Stack);
 ensures {:atomic} |{ A: Stack := Add(Stack, x, TopOfStack); TopOfStack := x; return true; }|;
 {
   var t: Node;
@@ -61,30 +61,30 @@ ensures {:atomic} |{ A: Stack := Add(Stack, x, TopOfStack); TopOfStack := x; ret
   var {:linear "Node"} t_lmap: lmap;
 
   yield;
-  assert {:phase 1} Inv(TopOfStack, Stack);
+  assert {:layer 1} Inv(TopOfStack, Stack);
   t_lmap := x_lmap;
   while (true)
-  invariant {:phase 1} dom(t_lmap) == dom(x_lmap);
-  invariant {:phase 1} Inv(TopOfStack, Stack);
+  invariant {:layer 1} dom(t_lmap) == dom(x_lmap);
+  invariant {:layer 1} Inv(TopOfStack, Stack);
   {
     call t := ReadTopOfStack();
     call t_lmap := Store(t_lmap, x, t);
     call g, t_lmap := TransferToStack(t, x, t_lmap); 
     if (g) {
-      assert {:phase 1} map(Stack)[x] == t;
+      assert {:layer 1} map(Stack)[x] == t;
       break;
     }
     yield; 
-    assert {:phase 1} dom(t_lmap) == dom(x_lmap);
-    assert {:phase 1} Inv(TopOfStack, Stack);
+    assert {:layer 1} dom(t_lmap) == dom(x_lmap);
+    assert {:layer 1} Inv(TopOfStack, Stack);
   }
   yield; 
-  assert {:expand} {:phase 1} Inv(TopOfStack, Stack);
+  assert {:expand} {:layer 1} Inv(TopOfStack, Stack);
 }
 
-procedure {:yields} {:phase 1} pop()
-requires {:phase 1} Inv(TopOfStack, Stack);
-ensures {:phase 1} Inv(TopOfStack, Stack);
+procedure {:yields} {:layer 1} pop()
+requires {:layer 1} Inv(TopOfStack, Stack);
+ensures {:layer 1} Inv(TopOfStack, Stack);
 ensures {:atomic} |{ var t: Node; 
                      A: assume TopOfStack != null; t := TopOfStack; Used := Add(Used, t, map(Stack)[t]); TopOfStack := map(Stack)[t]; Stack := Remove(Stack, t); return true; }|;
 {
@@ -93,9 +93,9 @@ ensures {:atomic} |{ var t: Node;
   var t: Node;
 
   yield;
-  assert {:phase 1} Inv(TopOfStack, Stack);
+  assert {:layer 1} Inv(TopOfStack, Stack);
   while (true)
-  invariant {:phase 1} Inv(TopOfStack, Stack);
+  invariant {:layer 1} Inv(TopOfStack, Stack);
   {
     call t := ReadTopOfStack();
     if (t != null) {
@@ -106,10 +106,10 @@ ensures {:atomic} |{ var t: Node;
       }
     }
     yield;
-    assert {:phase 1} Inv(TopOfStack, Stack);
+    assert {:layer 1} Inv(TopOfStack, Stack);
   }
   yield;
-  assert {:phase 1} Inv(TopOfStack, Stack);
+  assert {:layer 1} Inv(TopOfStack, Stack);
 }
 
 function Equal([int]bool, [int]bool) returns (bool);
